simulations/simglobal/SimGlobal.v
@@ -9,7 +9,6 @@ Require Import PCM.
 Require Import Coq.Relations.Relation_Definitions.
 Require Import Relation_Operators.
 Require Import RelationPairs.
-From Ordinal Require Import Ordinal Arithmetic.
 Require Import SimSTS.
 
 Set Implicit Arguments.
